compiler/yul/Counter.yul
@@ -8,16 +8,25 @@ object "Counter" {
             switch shr(224, calldataload(0))
             case 0xd09de08a {
                 /* increment() */
+                if callvalue() {
+                    revert(0, 0)
+                }
                 sstore(0, add(sload(0), 1))
                 stop()
             }
             case 0x2baeceb7 {
                 /* decrement() */
+                if callvalue() {
+                    revert(0, 0)
+                }
                 sstore(0, sub(sload(0), 1))
                 stop()
             }
             case 0xa87d942c {
                 /* getCount() */
+                if callvalue() {
+                    revert(0, 0)
+                }
                 mstore(0, sload(0))
                 return(0, 32)
             }
