compiler/yul/Ledger.yul
@@ -13,6 +13,9 @@ object "Ledger" {
             switch shr(224, calldataload(0))
             case 0xb6b55f25 {
                 /* deposit() */
+                if callvalue() {
+                    revert(0, 0)
+                }
                 let amount := calldataload(4)
                 let senderBal := sload(mappingSlot(0, caller()))
                 sstore(mappingSlot(0, caller()), add(senderBal, amount))
@@ -20,6 +23,9 @@ object "Ledger" {
             }
             case 0x2e1a7d4d {
                 /* withdraw() */
+                if callvalue() {
+                    revert(0, 0)
+                }
                 let amount := calldataload(4)
                 let senderBal := sload(mappingSlot(0, caller()))
                 if lt(senderBal, amount) {
@@ -34,6 +40,9 @@ object "Ledger" {
             }
             case 0xa9059cbb {
                 /* transfer() */
+                if callvalue() {
+                    revert(0, 0)
+                }
                 let to := and(calldataload(4), 0xffffffffffffffffffffffffffffffffffffffff)
                 let amount := calldataload(36)
                 let senderBal := sload(mappingSlot(0, caller()))
@@ -62,6 +71,9 @@ object "Ledger" {
             }
             case 0xf8b2cb4f {
                 /* getBalance() */
+                if callvalue() {
+                    revert(0, 0)
+                }
                 let addr := and(calldataload(4), 0xffffffffffffffffffffffffffffffffffffffff)
                 mstore(0, sload(mappingSlot(0, addr)))
                 return(0, 32)
