compiler/yul/SimpleToken.yul
@@ -18,6 +18,9 @@ object "SimpleToken" {
             switch shr(224, calldataload(0))
             case 0x40c10f19 {
                 /* mint() */
+                if callvalue() {
+                    revert(0, 0)
+                }
                 let to := and(calldataload(4), 0xffffffffffffffffffffffffffffffffffffffff)
                 let amount := calldataload(36)
                 if iszero(eq(caller(), sload(0))) {
@@ -51,6 +54,9 @@ object "SimpleToken" {
             }
             case 0xa9059cbb {
                 /* transfer() */
+                if callvalue() {
+                    revert(0, 0)
+                }
                 let to := and(calldataload(4), 0xffffffffffffffffffffffffffffffffffffffff)
                 let amount := calldataload(36)
                 let senderBal := sload(mappingSlot(1, caller()))
@@ -79,17 +85,26 @@ object "SimpleToken" {
             }
             case 0x70a08231 {
                 /* balanceOf() */
+                if callvalue() {
+                    revert(0, 0)
+                }
                 let addr := and(calldataload(4), 0xffffffffffffffffffffffffffffffffffffffff)
                 mstore(0, sload(mappingSlot(1, addr)))
                 return(0, 32)
             }
             case 0x18160ddd {
                 /* totalSupply() */
+                if callvalue() {
+                    revert(0, 0)
+                }
                 mstore(0, sload(2))
                 return(0, 32)
             }
             case 0x8da5cb5b {
                 /* owner() */
+                if callvalue() {
+                    revert(0, 0)
+                }
                 mstore(0, sload(0))
                 return(0, 32)
             }
